test-suite/Congruence/AlgoBool.v
@@ -1,0 +1,216 @@
+(** Congruence closure *)
+Require Import Arith.Peano_dec.
+Require Import List.
+Require Import Coqbottom.
+Require Import Coqbottom.Map.
+Require Import Coqbottom.DataStructures.
+Require Import Definitions.
+
+Set Implicit Arguments.
+Set Transparent Obligation.
+Import Monad ListNotations.
+
+(** The congruence-closure algorithm returning only a proof of [True] *)
+Module CongruenceClosureBool (P: Parameters).
+  (** Fake [EqProof] to compute the time lost in proof computations *)
+  Module EqProof.
+    Record t (T: Type) (values: Values.t T) := Make {
+      i: Index.t;
+      j: Index.t;
+      H: True}.
+    
+    Arguments Make [T values i j] H.
+  End EqProof.
+  
+  Definition T: Type := EqProof.t P.Values.
+  
+  Definition Sig: Sig.t := Sig.Make nil
+    (Index.FMap.t T :: (bool: Type) :: nil).
+  
+  Definition Hash := Ref.t Sig (Index.FMap.t T).
+  Definition M := M Sig.
+  
+  Definition read (hash: Hash) (key: Index.t): M T :=
+    let! map := !hash in
+    match Index.FMap.find key map with
+    | None => error "Hash read: not found"
+    | Some v => ret v
+    end.
+  
+  Definition write (hash: Hash) (key: Index.t) (value: T): M unit :=
+    let! map := !hash in
+    match Index.FMap.find key map with
+    | None => error "Hash write: not found"
+    | Some _ => hash :=! Index.FMap.add key value map
+    end.
+  
+  Definition do (map: Index.FMap.t (M unit)): M (Index.FMap.t unit) :=
+    Index.FMap.fold (fun k x map' =>
+      let! x := x in
+      let! map' := map' in
+      ret (Index.FMap.add k x map'))
+      map (ret (Index.FMap.empty _)).
+  
+  Definition iter (hash: Hash) (f: Index.t -> T -> M unit): M unit :=
+    let! map := !hash in
+    do! do (Index.FMap.mapi f map) in
+    ret tt.
+  
+  Definition Find (hash: Hash) (index: Index.t)
+    : M {index': Index.t | True}.
+    refine (
+      dependent_fix (fun i => {j: Index.t | True})
+        (fun f i =>
+          let! eq_proof := read hash i in
+          let (i', j, Hij) := eq_proof in
+          match Index.eqb i i' with
+            | true => _
+            | false => error "Find: i <> i' unexpected"
+          end)
+        index).
+    refine (
+      match Index.eqb i j with
+        | true => ret (exist _ j _)
+        | false =>
+          let! r := f j in
+          let (k, Hjk) := r in
+          do! write hash i (EqProof.Make (i := i) (j := k) _) in
+          ret (exist _ k _)
+      end); exact I.
+  Defined.
+  
+  (** Do the union and return [true] if the values were in different sets *)
+  Definition Merge (hash: Hash) (Hij: T): M bool.
+    refine (
+      let (i, j, Hij) := Hij in
+      let! Pii' := Find hash i in
+      let! Pjj' := Find hash j in
+      let (i', Hii') := Pii' in
+      let (j', Hjj') := Pjj' in
+      match Index.eqb i' j' with
+      | true => ret false
+      | false =>
+        do! write hash i' (EqProof.Make (i := i') (j := j') _) in
+        ret true
+      end); exact I.
+  Defined.
+  
+  (** The equality proof of two values if they are equivalent *)
+  Definition AreEquiv (hash: Hash) (i j: Index.t)
+    : M (option True).
+    refine (
+      let! Pii' := Find hash i in
+      let! Pjj' := Find hash j in
+      let (i', Hii') := Pii' in
+      let (j', Hjj') := Pjj' in
+      match Index.eqb i' j' with
+      | true => ret (Some _)
+      | false => ret None
+      end);
+    exact I.
+  Defined.
+  
+  Fixpoint areCongruentAux (xs ys: list Index.t)
+    (f: forall (x y: Index.t), M (option True))
+    {struct xs}
+    : M (option True).
+    destruct xs as [| x xs]; destruct ys as [| y ys];
+      [exact (ret (Some I)) | exact (ret None) |
+      exact (ret None) | ]; simpl.
+    refine (
+      let! Pxy := f x y in
+      let! Pxsys := areCongruentAux xs ys f in
+      match (Pxy, Pxsys) with
+      | (Some _, Some _) => ret (Some _)
+      | _ => ret None
+      end); exact I.
+  Defined.
+  
+  (** The equality proof of two values if they are congruent *)
+  Definition AreCongruent (hash: Hash)
+    : forall (ij: Index.t * Index.t),
+      M (option True).
+    refine (dependent_fix
+      (fun xy => option True)
+      _); intros f xy.
+    destruct xy as [x y].
+    refine (
+      let! OHxy := AreEquiv hash x y in
+      match OHxy with
+      | Some _ => ret OHxy
+      | None => _
+      end); clear OHxy.
+    destruct x as [i xs]; destruct y as [j ys]; simpl.
+    refine (
+      match NPeano.Nat.eqb i j with
+      | true =>
+        let! OHxsys := areCongruentAux xs ys (fun x y => f (x, y)) in
+        match OHxsys with
+        | None => ret None
+        | Some Hxsys => ret (Some _)
+        end
+      | false => ret None
+      end); exact I.
+  Defined.
+  
+  (** Merge two equal values and merge the new congruent terms *)
+  Definition RecurseMerge (hash: Hash) (get_preds: Index.t -> M Index.FSet.t)
+    (Pij: T): M bool :=
+    fix_ (fun recurse_merge Pij =>
+      let! b := Merge hash Pij in
+      if b then
+        let (i, j, _) := Pij in
+        let! ps := get_preds i in
+        let! qs := get_preds j in
+        do!
+          Index.FSet.fold (fun p next =>
+            do! next in
+            Index.FSet.fold (fun q next =>
+              do! next in
+              let! P := AreCongruent hash (p, q) in
+              match P with
+              | Some P =>
+                do! recurse_merge (EqProof.Make (i := p) (j := q) P) in
+                ret tt
+              | None => ret tt
+              end)
+              qs (ret tt))
+            ps (ret tt) in
+        ret true
+      else
+        ret false)
+      Pij.
+  
+  (** Generate the congruent relation given a list of equalities and
+      other involved terms *)
+  Definition CongruenceClosure (eq_proofs: list T) (other_indexes: list Index.t)
+    : M Hash :=
+    let preds :=
+      Index.Preds (other_indexes ++ flat_map (fun (P: T) =>
+        let (i, j, _) := P in
+        i :: j :: nil) eq_proofs) in
+    let get_preds (i: Index.t): M Index.FSet.t :=
+      match Index.FMap.find i preds with
+      | Some s => ret s
+      | None => error "Invalid index in preds"
+      end in
+    let! hash := tmp_ref Sig 0 (Index.FMap.mapi (fun i _ =>
+      EqProof.Make (i := i) (j := i) I) preds) in
+    do! List.do (List.map (RecurseMerge hash get_preds) eq_proofs) in
+    ret hash.
+  
+  (** Compute the equality proof of two terms with congruence-closure *)
+  Definition ProveEqual (eq_proofs: list T) (i j: Index.t)
+    : M True.
+    refine (
+      let! hash := CongruenceClosure eq_proofs (i :: j :: nil) in
+      let! Pii' := Find hash i in
+      let! Pjj' := Find hash j in
+      let (i', Hii') := Pii' in
+      let (j', Hjj') := Pjj' in
+      match Index.eqb i' j' with
+      | true => ret _
+      | false => error "Equality proof not found"
+      end); exact I.
+  Defined.
+End CongruenceClosureBool.
